Lean4bits/lemmas.lean
@@ -1,5 +1,10 @@
 import Mathlib.Data.Fintype.Card
+import Mathlib.Data.Fintype.Sum
+import Mathlib.Data.Fintype.Sigma
+import Mathlib.Data.Fintype.Pi
 import Lean4bits.defs
+import Mathlib.Tactic.Zify
+import Mathlib.Tactic.Ring
 
 open Sum
 
@@ -178,7 +183,7 @@ open Term
 | (var n) => n+1
 | zero => 0
 | one => 0
-| neg_one => 0
+| negOne => 0
 | Term.and t₁ t₂ => max (arity t₁) (arity t₂)
 | Term.or t₁ t₂ => max (arity t₁) (arity t₂)
 | Term.xor t₁ t₂ => max (arity t₁) (arity t₂)
@@ -194,7 +199,7 @@ open Term
 | var n, vars => vars (Fin.last n)
 | zero, _vars => zeroSeq
 | one, _vars => oneSeq
-| neg_one, _vars => negOneSeq
+| negOne, _vars => negOneSeq
 | Term.and t₁ t₂, vars =>
   andSeq (Term.evalFin t₁
     (fun i => vars (Fin.castLe (by simp [arity]) i)))
@@ -269,713 +274,648 @@ lemma not_eq_propagate (x : ℕ → Bool) :
   ext n; cases n <;> simp [propagate, propagateAux, notSeq]
 
 lemma ls_eq_propagate (x : ℕ → Bool) :
-  lsSeq x = propagate (λ _ : Unit => false) (λ (carry x : Unit → Bool) => (x, carry ())) (λ _ => x) :=
-begin
-  ext n,
-  cases n with n,
-  { refl },
-  { cases n,
-    { simp [lsSeq, propagate_succ] },
-    { simp [lsSeq, propagate_succ] } }
-end
+    lsSeq x = propagate (λ _ : Unit => false)
+      (λ (carry x : Unit → Bool) => (x, carry ())) (λ _ => x) := by
+  ext n
+  match n with
+  | 0 => rfl
+  | 1 => rfl
+  | n+2 => simp [lsSeq, propagate_succ]
 
-lemma add_seqAux_eq_propagateCarry (x y : ℕ → Bool) (n : ℕ) :
-  (add_seqAux x y n).2 = propagateCarry (λ _, false)
-    (λ (carry : Unit → Bool) (bits : Bool → Bool),
-      λ _, (bits true && bits false) || (bits false && carry ()) || (bits true && carry ()))
-  (λ b, cond b x y) n () :=
-begin
-  induction n,
-  { simp [add_seqAux] },
-  { simp [add_seqAux, *] }
-end
+lemma addSeqAux_eq_propagateCarry (x y : ℕ → Bool) (n : ℕ) :
+    (addSeqAux x y n).2 = propagateCarry (λ _ => false)
+      (λ (carry : Unit → Bool) (bits : Bool → Bool) =>
+        λ _ => (bits true && bits false) || (bits false && carry ()) || (bits true && carry ()))
+    (λ b => cond b x y) n () := by
+  induction n <;> simp [addSeqAux, *]
 
 lemma add_eq_propagate (x y : ℕ → Bool) :
-  add_seq x y = propagate (λ _, false)
-    (λ (carry : Unit → Bool) (bits : Bool → Bool),
-      (λ _, (bits true && bits false) || (bits false && carry ()) || (bits true && carry ()),
-        bxor (bits true) (bxor (bits false) (carry ()))))
-  (λ b, cond b x y) :=
-begin
-  ext n,
-  cases n with n,
-  { simp [add_seq, add_seqAux] },
-  { cases n,
-    { simp [add_seq, add_seqAux, propagate_succ] },
-    { simp [add_seq, add_seqAux, add_seqAux_eq_propagateCarry,
-        propagate_succ] } }
-end
+    addSeq x y = propagate (λ _ => false)
+      (λ (carry : Unit → Bool) (bits : Bool → Bool) =>
+        (λ _ => (bits true && bits false) || (bits false && carry ()) || (bits true && carry ()),
+          _root_.xor (bits true) (_root_.xor (bits false) (carry ()))))
+    (λ b => cond b x y) := by
+  ext n
+  match n with
+  | 0 => simp [addSeq, addSeqAux]
+  | 1 => simp [addSeq, addSeqAux, propagate, propagateAux]
+  | n+2 => simp [addSeq, addSeqAux, addSeqAux_eq_propagateCarry, propagate_succ]
 
-lemma sub_seqAux_eq_propagateCarry (x y : ℕ → Bool) (n : ℕ) :
-  (sub_seqAux x y n).2 = propagateCarry (λ _, false)
-    (λ (carry : Unit → Bool) (bits : Bool → Bool),
-      λ _, (bnot (bits true) && (bits false)) ||
-        (bnot (bxor (bits true) (bits false))) && carry ())
-  (λ b, cond b x y) n () :=
-begin
-  induction n,
-  { simp [sub_seqAux] },
-  { simp [sub_seqAux, *] }
-end
+lemma subSeqAux_eq_propagateCarry (x y : ℕ → Bool) (n : ℕ) :
+    (subSeqAux x y n).2 = propagateCarry (λ _ => false)
+      (λ (carry : Unit → Bool) (bits : Bool → Bool) =>
+        λ _ => (!(bits true) && (bits false)) ||
+          (!(_root_.xor (bits true) (bits false))) && carry ())
+    (λ b => cond b x y) n () := by
+  induction n <;> simp [subSeqAux, *]
 
 lemma sub_eq_propagate (x y : ℕ → Bool) :
-  sub_seq x y = propagate (λ _, false)
-    (λ (carry : Unit → Bool) (bits : Bool → Bool),
-      (λ _, (bnot (bits true) && (bits false)) ||
-        ((bnot (bxor (bits true) (bits false))) && carry ()),
-        bxor (bits true) (bxor (bits false) (carry ()))))
-  (λ b, cond b x y) :=
-begin
-  ext n,
-  cases n with n,
-  { simp [sub_seq, sub_seqAux] },
-  { cases n,
-    { simp [sub_seq, sub_seqAux, propagate_succ] },
-    { simp [sub_seq, sub_seqAux, sub_seqAux_eq_propagateCarry,
-        propagate_succ] } }
-end
+    subSeq x y = propagate (λ _ => false)
+      (λ (carry : Unit → Bool) (bits : Bool → Bool) =>
+        (λ _ => (!(bits true) && (bits false)) ||
+          ((!(_root_.xor (bits true) (bits false))) && carry ()),
+          _root_.xor (bits true) (_root_.xor (bits false) (carry ()))))
+    (λ b => cond b x y) := by
+  ext n
+  match n with
+  | 0 => simp [subSeq, subSeqAux]
+  | 1 => simp [subSeq, subSeqAux, propagate, propagateAux]
+  | n+2 => simp [subSeq, subSeqAux, subSeqAux_eq_propagateCarry, propagate_succ]
 
 lemma negSeqAux_eq_propagateCarry (x : ℕ → Bool) (n : ℕ) :
-  (negSeqAux x n).2 = propagateCarry (λ _, true)
-    (λ (carry : Unit → Bool) (bits : Unit → Bool),
-      λ _, (bnot (bits ())) && (carry ()))
-  (λ _, x) n () :=
-begin
-  induction n,
-  { simp [negSeqAux] },
-  { simp [negSeqAux, *] }
-end
+    (negSeqAux x n).2 = propagateCarry (λ _ => true)
+      (λ (carry : Unit → Bool) (bits : Unit → Bool) =>
+        λ _ => (!(bits ())) && (carry ()))
+    (λ _ => x) n () := by
+  induction n <;> simp [negSeqAux, *]
 
 lemma neg_eq_propagate (x : ℕ → Bool) :
-  negSeq x = propagate (λ _, true)
-    (λ (carry : Unit → Bool) (bits : Unit → Bool),
-      (λ _, (bnot (bits ())) && (carry ()), bxor (bnot (bits ())) (carry ())))
-  (λ _, x) :=
-begin
-  ext n,
-  cases n with n,
-  { simp [negSeq, negSeqAux] },
-  { cases n,
-    { simp [negSeq, negSeqAux, propagate_succ] },
-    { simp [negSeq, negSeqAux, negSeqAux_eq_propagateCarry,
-        propagate_succ] } }
-end
+    negSeq x = propagate (λ _ => true)
+      (λ (carry : Unit → Bool) (bits : Unit → Bool) =>
+        (λ _ => (!(bits ())) && (carry ()), _root_.xor (!(bits ())) (carry ())))
+    (λ _ => x) := by
+  ext n
+  match n with
+  | 0 => simp [negSeq, negSeqAux]
+  | 1 => simp [negSeq, negSeqAux, propagate, propagateAux]
+  | n+2 => simp [negSeq, negSeqAux, negSeqAux_eq_propagateCarry, propagate_succ]
 
 lemma incrSeqAux_eq_propagateCarry (x : ℕ → Bool) (n : ℕ) :
-  (incrSeqAux x n).2 = propagateCarry (λ _, true)
-    (λ (carry : Unit → Bool) (bits : Unit → Bool),
-      λ _, (bits ()) && carry ())
-  (λ _, x) n () :=
-begin
-  induction n,
-  { simp [incrSeqAux] },
-  { simp [incrSeqAux, *] }
-end
+    (incrSeqAux x n).2 = propagateCarry (λ _ => true)
+      (λ (carry : Unit → Bool) (bits : Unit → Bool) =>
+        λ _ => (bits ()) && carry ())
+    (λ _ => x) n () := by
+  induction n <;> simp [incrSeqAux, *]
 
 lemma incr_eq_propagate (x : ℕ → Bool) :
-  incrSeq x = propagate (λ _, true)
-    (λ (carry : Unit → Bool) (bits : Unit → Bool),
-      (λ _, (bits ()) && carry (), bxor (bits ()) (carry ())))
-  (λ _, x) :=
-begin
-  ext n,
-  cases n with n,
-  { simp [incrSeq, incrSeqAux] },
-  { cases n,
-    { simp [incrSeq, incrSeqAux, propagate_succ] },
-    { simp [incrSeq, incrSeqAux, incrSeqAux_eq_propagateCarry,
-        propagate_succ] } }
-end
+    incrSeq x = propagate (λ _ => true)
+      (λ (carry : Unit → Bool) (bits : Unit → Bool) =>
+        (λ _ => (bits ()) && carry (), _root_.xor (bits ()) (carry ())))
+    (λ _ => x) := by
+  ext n
+  match n with
+  | 0 => simp [incrSeq, incrSeqAux]
+  | 1 => simp [incrSeq, incrSeqAux, propagate, propagateAux]
+  | n+2 => simp [incrSeq, incrSeqAux, incrSeqAux_eq_propagateCarry, propagate_succ]
 
 lemma decrSeqAux_eq_propagateCarry (x : ℕ → Bool) (n : ℕ) :
-  (decrSeqAux x n).2 = propagateCarry (λ _, true)
-    (λ (carry : Unit → Bool) (bits : Unit → Bool),
-      λ _, (bnot (bits ())) && carry ())
-  (λ _, x) n () :=
-begin
-  induction n,
-  { simp [decrSeqAux] },
-  { simp [decrSeqAux, *] }
-end
+    (decrSeqAux x n).2 = propagateCarry (λ _ => true)
+      (λ (carry : Unit → Bool) (bits : Unit → Bool) =>
+        λ _ => (!(bits ())) && carry ())
+    (λ _ => x) n () := by
+  induction n <;> simp [decrSeqAux, *]
 
 lemma decr_eq_propagate (x : ℕ → Bool) :
-  decrSeq x = propagate (λ _, true)
-    (λ (carry : Unit → Bool) (bits : Unit → Bool),
-      (λ _, (bnot (bits ())) && carry (), bxor (bits ()) (carry ())))
-  (λ _, x) :=
-begin
-  ext n,
-  cases n with n,
-  { simp [decrSeq, decrSeqAux] },
-  { cases n,
-    { simp [decrSeq, decrSeqAux, propagate_succ] },
-    { simp [decrSeq, decrSeqAux, decrSeqAux_eq_propagateCarry,
-        propagate_succ] } }
-end
+    decrSeq x = propagate (λ _ => true)
+      (λ (carry : Unit → Bool) (bits : Unit → Bool) =>
+        (λ _ => (!(bits ())) && carry (), _root_.xor (bits ()) (carry ())))
+    (λ _ => x) := by
+  ext n
+  match n with
+  | 0 => simp [decrSeq, decrSeqAux]
+  | 1 => simp [decrSeq, decrSeqAux, propagate, propagateAux]
+  | n+2 => simp [decrSeq, decrSeqAux, decrSeqAux_eq_propagateCarry, propagate_succ]
 
-structure propagate_struc (arity : Type) : Type 1 :=
-( α  : Type )
-[ i : Fintype α ]
-( init_carry : α → Bool )
-( next_bit : ∀ (carry : α → Bool) (bits : arity → Bool),
-    (α → Bool) × Bool )
+structure PropagateStruc (arity : Type) : Type 1 :=
+  ( α  : Type )
+  [ i : Fintype α ]
+  ( init_carry : α → Bool )
+  ( next_bit : ∀ (_carry : α → Bool) (_bits : arity → Bool),
+      (α → Bool) × Bool )
 
-atrueribute [instance] propagate_struc.i
+attribute [instance] PropagateStruc.i
 
-namespace propagate_struc
+namespace PropagateStruc
 
-variables {arity : Type} (p : propagate_struc arity)
+variable {arity : Type} (p : PropagateStruc arity)
 
 def eval : (arity → ℕ → Bool) → ℕ → Bool :=
-propagate p.init_carry p.next_bit
+  propagate p.init_carry p.next_bit
 
 def changeVars {arity2 : Type} (changeVars : arity → arity2) :
-  propagate_struc arity2 :=
-{ α := p.α,
-  i := p.i,
-  init_carry := p.init_carry,
-  next_bit := λ carry bits, p.next_bit carry (fun i => bits (changeVars i)) }
+    PropagateStruc arity2 :=
+  { α := p.α,
+    i := p.i,
+    init_carry := p.init_carry,
+    next_bit := λ carry bits => p.next_bit carry (fun i => bits (changeVars i)) }
 
-def compose [fintype arity]
+def compose [Fintype arity]
   (new_arity : Type)
-  (q_arity : arity → Type)
-  (vars : ∀ (a : arity), q_arity a → new_arity)
-  (q : ∀ (a : arity), propagate_struc (q_arity a)) :
-  propagate_struc (new_arity) :=
-{ α := p.α ⊕ (Σ a, (q a).α),
-  i := by letI := p.i; apply_instance,
-  init_carry := Sum.elim p.init_carry (λ x, (q x.1).init_carry x.2),
-  next_bit := λ carry bits,
-    let f : ∀ (a : arity), ((q a).α → Bool) × Bool := λ a, (q a).next_bit (λ d,
-        carry (inr ⟨a, d⟩)) (λ d, bits (vars a d)) in
-    let g : (p.α → Bool) × Bool := (p.next_bit (carry ∘ inl) (λ a, (f a).2)) in
-    (Sum.elim g.1 (λ x, (f x.1).1 x.2), g.2) }
+    (q_arity : arity → Type)
+    (vars : ∀ (a : arity), q_arity a → new_arity)
+    (q : ∀ (a : arity), PropagateStruc (q_arity a)) :
+    PropagateStruc (new_arity) :=
+  { α := p.α ⊕ (Σ a, (q a).α),
+    i := by letI := p.i;  infer_instance,
+    init_carry := Sum.elim p.init_carry (λ x => (q x.1).init_carry x.2),
+    next_bit := λ carry bits =>
+      let f : ∀ (a : arity), ((q a).α → Bool) × Bool := λ a => (q a).next_bit (λ d =>
+          carry (inr ⟨a, d⟩)) (λ d => bits (vars a d))
+      let g : (p.α → Bool) × Bool := (p.next_bit (carry ∘ inl) (λ a => (f a).2))
+      (Sum.elim g.1 (λ x => (f x.1).1 x.2), g.2) }
 
-lemma eval_compose [fintype arity]
-  (new_arity : Type)
-  (q_arity : arity → Type)
-  (vars : ∀ (a : arity), q_arity a → new_arity)
-  (q : ∀ (a : arity), propagate_struc (q_arity a))
-  (x : new_arity → ℕ → Bool):
-  (p.compose new_arity q_arity vars q).eval x =
-  p.eval (λ a, (q a).eval (fun i => x (vars _ i))) :=
-begin
-  ext n,
-  simp only [eval, compose, propagate_propagate]
-end
+lemma eval_compose [Fintype arity]
+    (new_arity : Type)
+    (q_arity : arity → Type)
+    (vars : ∀ (a : arity), q_arity a → new_arity)
+    (q : ∀ (a : arity), PropagateStruc (q_arity a))
+    (x : new_arity → ℕ → Bool):
+    (p.compose new_arity q_arity vars q).eval x =
+    p.eval (λ a => (q a).eval (fun i => x (vars _ i))) := by
+  ext n; simp only [eval, compose, propagate_propagate]
 
-def and : propagate_struc Bool :=
-{ α := empty,
-  i := by apply_instance,
+
+def and : PropagateStruc Bool :=
+  { α := Empty,
+    i := by infer_instance,
+    init_carry := Empty.elim,
+    next_bit := λ _carry bits => (Empty.elim, bits true && bits false) }
+
+@[simp] lemma eval_and (x : Bool → ℕ → Bool) : and.eval x = andSeq (x true) (x false) := by
+  ext n; cases n <;> simp [and, andSeq, eval, propagate_succ]
+
+def or : PropagateStruc Bool :=
+  { α := Empty,
+    i := by infer_instance,
+    init_carry := Empty.elim,
+    next_bit := λ _carry bits => (Empty.elim, bits true || bits false) }
+
+@[simp] lemma eval_or (x : Bool → ℕ → Bool) : or.eval x = orSeq (x true) (x false) := by
+  ext n; cases n <;> simp [or, orSeq, eval, propagate_succ]
+
+def xor : PropagateStruc Bool :=
+  { α := Empty,
+    i := by infer_instance,
+    init_carry := Empty.elim,
+    next_bit := λ _carry bits => (Empty.elim, _root_.xor (bits true) (bits false)) }
+
+@[simp] lemma eval_xor (x : Bool → ℕ → Bool) : xor.eval x = xorSeq (x true) (x false) := by
+  ext n; cases n <;> simp [xor, xorSeq, eval, propagate_succ]
+
+  def add : PropagateStruc Bool :=
+  { α := Unit,
+    i := by infer_instance,
+    init_carry := λ _ => false,
+    next_bit := λ (carry : Unit → Bool) (bits : Bool → Bool) =>
+        (λ _ => (bits true && bits false) || (bits false && carry ()) || (bits true && carry ()),
+          _root_.xor (bits true) (_root_.xor (bits false) (carry ()))) }
+
+@[simp] lemma eval_add (x : Bool → ℕ → Bool) : add.eval x = addSeq (x true) (x false) := by
+  dsimp [add, eval]
+  rw [add_eq_propagate]
+  congr
+  funext b
+  cases b; rfl
+  simp
+  congr
+  funext i
+  cases i <;> simp
+
+
+def sub : PropagateStruc Bool :=
+  { α := Unit,
+    i := by infer_instance,
+    init_carry := λ _ => false,
+    next_bit := λ (carry : Unit → Bool) (bits : Bool → Bool) =>
+        (λ _ => (!(bits true) && (bits false)) ||
+          ((!(_root_.xor (bits true) (bits false))) && carry ()),
+          _root_.xor (bits true) (_root_.xor (bits false) (carry ()))) }
+
+@[simp] lemma eval_sub (x : Bool → ℕ → Bool) : sub.eval x = subSeq (x true) (x false) := by
+  dsimp [sub, eval]
+  rw [sub_eq_propagate]
+  congr
+  funext b
+  cases b;  rfl
+  simp
+  congr
+  funext i
+  cases i <;> simp
+
+def neg : PropagateStruc Unit :=
+  { α := Unit,
+    i := by infer_instance,
+    init_carry := λ _ => true,
+    next_bit := λ (carry : Unit → Bool) (bits : Unit → Bool) =>
+      (λ _ => (!(bits ())) && (carry ()), _root_.xor (!(bits ())) (carry ())) }
+
+@[simp] lemma eval_neg (x : Unit → ℕ → Bool) : neg.eval x = negSeq (x ()) := by
+  dsimp [neg, eval]
+  rw [neg_eq_propagate]
+
+def not : PropagateStruc Unit :=
+{ α := Empty,
+  i := by infer_instance,
   init_carry := Empty.elim,
-  next_bit := λ carry bits, (Empty.elim, bits true && bits false) }
+  next_bit := λ _carry bits => (Empty.elim, !(bits ())) }
 
-@[simp] lemma eval_and (x : Bool → ℕ → Bool) : and.eval x = andSeq (x true) (x false) :=
-by ext n; cases n; simp [and, andSeq, eval, propagate_succ]
+@[simp] lemma eval_not (x : Unit → ℕ → Bool) : not.eval x = notSeq (x ()) := by
+  ext n; cases n <;> simp [not, notSeq, eval, propagate_succ]
 
-def or : propagate_struc Bool :=
-{ α := empty,
-  i := by apply_instance,
-  init_carry := Empty.elim,
-  next_bit := λ carry bits, (Empty.elim, bits true || bits false) }
+def zero : PropagateStruc (Fin 0) :=
+  { α := Empty,
+    i := by infer_instance,
+    init_carry := Empty.elim,
+    next_bit := λ _carry _bits => (Empty.elim, false) }
 
-@[simp] lemma eval_or (x : Bool → ℕ → Bool) : or.eval x = orSeq (x true) (x false) :=
-by ext n; cases n; simp [or, orSeq, eval, propagate_succ]
+@[simp] lemma eval_zero (x : Fin 0 → ℕ → Bool) : zero.eval x = zeroSeq := by
+  ext n; cases n <;> simp [zero, zeroSeq, eval, propagate_succ]
 
-def xor : propagate_struc Bool :=
-{ α := empty,
-  i := by apply_instance,
-  init_carry := Empty.elim,
-  next_bit := λ carry bits, (Empty.elim, bxor (bits true) (bits false)) }
+def one : PropagateStruc (Fin 0) :=
+  { α := Unit,
+    i := by infer_instance,
+    init_carry := λ _ => true,
+    next_bit := λ carry _bits => (λ _ => false, carry ()) }
 
-@[simp] lemma eval_xor (x : Bool → ℕ → Bool) : xor.eval x = xorSeq (x true) (x false) :=
-by ext n; cases n; simp [xor, xorSeq, eval, propagate_succ]
+@[simp] lemma eval_one (x : Fin 0 → ℕ → Bool) : one.eval x = oneSeq := by
+  ext n; cases n <;> simp [one, oneSeq, eval, propagate_succ2, @eq_comm _ false]
 
-def add : propagate_struc Bool :=
-{ α := Unit,
-  i := by apply_instance,
-  init_carry := λ _, false,
-  next_bit := λ (carry : Unit → Bool) (bits : Bool → Bool),
-      (λ _, (bits true && bits false) || (bits false && carry ()) || (bits true && carry ()),
-        bxor (bits true) (bxor (bits false) (carry ()))) }
+def negOne : PropagateStruc (Fin 0) :=
+  { α := Empty,
+    i := by infer_instance,
+    init_carry := Empty.elim,
+    next_bit := λ _carry _bits => (Empty.elim, true) }
 
-@[simp] lemma eval_add (x : Bool → ℕ → Bool) : add.eval x = add_seq (x true) (x false) :=
-begin
-  dsimp [add, eval],
-  rw [add_eq_propagate],
-  congr,
-  funext b,
-  cases b; refl
-end
+@[simp] lemma eval_negOne (x : Fin 0 → ℕ → Bool) : negOne.eval x = negOneSeq := by
+  ext n; cases n <;> simp [negOne, negOneSeq, eval, propagate_succ2]
 
-def sub : propagate_struc Bool :=
-{ α := Unit,
-  i := by apply_instance,
-  init_carry := λ _, false,
-  next_bit := λ (carry : Unit → Bool) (bits : Bool → Bool),
-      (λ _, (bnot (bits true) && (bits false)) ||
-        ((bnot (bxor (bits true) (bits false))) && carry ()),
-        bxor (bits true) (bxor (bits false) (carry ()))) }
+def ls : PropagateStruc Unit :=
+  { α := Unit,
+    i := by infer_instance,
+    init_carry := λ _ => false,
+    next_bit := λ carry bits => (bits, carry ()) }
 
-@[simp] lemma eval_sub (x : Bool → ℕ → Bool) : sub.eval x = sub_seq (x true) (x false) :=
-begin
-  dsimp [sub, eval],
-  rw [sub_eq_propagate],
-  congr,
-  funext b,
-  cases b; refl
-end
+@[simp] lemma eval_ls (x : Unit → ℕ → Bool) : ls.eval x = lsSeq (x ()) := by
+  ext n; cases n <;> simp [ls, lsSeq, eval, propagate_succ2]
 
-def neg : propagate_struc Unit :=
-{ α := Unit,
-  i := by apply_instance,
-  init_carry := λ _, true,
-  next_bit := λ (carry : Unit → Bool) (bits : Unit → Bool),
-    (λ _, (bnot (bits ())) && (carry ()), bxor (bnot (bits ())) (carry ())) }
+def var (n : ℕ) : PropagateStruc (Fin (n+1)) :=
+  { α := Empty,
+    i := by infer_instance,
+    init_carry := Empty.elim,
+    next_bit := λ _carry bits => (Empty.elim, bits (Fin.last n)) }
 
-@[simp] lemma eval_neg (x : Unit → ℕ → Bool) : neg.eval x = negSeq (x ()) :=
-begin
-  dsimp [neg, eval],
-  rw [neg_eq_propagate],
-  congr,
-  funext b,
-  cases b; refl
-end
+@[simp] lemma eval_var (n : ℕ) (x : Fin (n+1) → ℕ → Bool) : (var n).eval x = x (Fin.last n) := by
+  ext m; cases m <;> simp [var, eval, propagate_succ]
 
-def not : propagate_struc Unit :=
-{ α := empty,
-  i := by apply_instance,
-  init_carry := Empty.elim,
-  next_bit := λ carry bits, (Empty.elim, bnot (bits ())) }
+def incr : PropagateStruc Unit :=
+  { α := Unit,
+    i := by infer_instance,
+    init_carry := λ _ => true,
+    next_bit := λ carry bits => (λ _ => bits () && carry (), _root_.xor (bits ()) (carry ())) }
 
-@[simp] lemma eval_not (x : Unit → ℕ → Bool) : not.eval x = notSeq (x ()) :=
-by ext n; cases n; simp [not, notSeq, eval, propagate_succ]
+@[simp] lemma eval_incr (x : Unit → ℕ → Bool) : incr.eval x = incrSeq (x ()) := by
+  dsimp [incr, eval]
+  rw [incr_eq_propagate]
 
-def zero : propagate_struc (fin 0) :=
-{ α := empty,
-  i := by apply_instance,
-  init_carry := Empty.elim,
-  next_bit := λ carry bits, (Empty.elim, false) }
+def decr : PropagateStruc Unit :=
+  { α := Unit,
+    i := by infer_instance,
+    init_carry := λ _ => true,
+    next_bit := λ carry bits => (λ _ => !(bits ()) && carry (), _root_.xor (bits ()) (carry ())) }
 
-@[simp] lemma eval_zero (x : Fin 0 → ℕ → Bool) : zero.eval x = zeroSeq :=
-by ext n; cases n; simp [zero, zeroSeq, eval, propagate_succ]
+@[simp] lemma eval_decr (x : Unit → ℕ → Bool) : decr.eval x = decrSeq (x ()) := by
+  dsimp [decr, eval]
+  rw [decr_eq_propagate]
 
-def one : propagate_struc (fin 0) :=
-{ α := Unit,
-  i := by apply_instance,
-  init_carry := λ _, true,
-  next_bit := λ carry bits, (λ _, false, carry ()) }
+end PropagateStruc
 
-@[simp] lemma eval_one (x : Fin 0 → ℕ → Bool) : one.eval x = oneSeq :=
-by ext n; cases n; simp [one, oneSeq, eval, propagate_succ2]
+structure PropagateSolution (t : Term) extends PropagateStruc (Fin (arity t)) :=
+( good : t.evalFin = toPropagateStruc.eval )
 
-def neg_one : propagate_struc (fin 0) :=
-{ α := empty,
-  i := by apply_instance,
-  init_carry := Empty.elim,
-  next_bit := λ carry bits, (Empty.elim, true) }
+def composeUnary
+    (p : PropagateStruc Unit)
+    {t : Term}
+    (q : PropagateSolution t) :
+    PropagateStruc (Fin (arity t)) :=
+  p.compose
+    (Fin (arity t))
+    _
+    (λ _ => id)
+    (λ _ => q.toPropagateStruc)
+def X := @Bool.casesOn
+def composeBinary
+    (p : PropagateStruc Bool)
+    {t₁ t₂ : Term}
+    (q₁ : PropagateSolution t₁)
+    (q₂ : PropagateSolution t₂) :
+    PropagateStruc (Fin (max (arity t₁) (arity t₂))) :=
+  p.compose (Fin (max (arity t₁) (arity t₂)))
+    (λ b => Fin (cond b (arity t₁) (arity t₂)))
+    (λ b i => Fin.castLe (by cases b <;> simp) i)
+    (λ b => match b with
+      | true => q₁.toPropagateStruc
+      | false => q₂.toPropagateStruc)
 
-@[simp] lemma eval_neg_one (x : Fin 0 → ℕ → Bool) : neg_one.eval x = neg_oneSeq :=
-by ext n; cases n; simp [neg_one, neg_oneSeq, eval, propagate_succ2]
+@[simp] lemma composeUnary_eval
+    (p : PropagateStruc Unit)
+    {t : Term}
+    (q : PropagateSolution t)
+    (x : Fin (arity t) → ℕ → Bool) :
+    (composeUnary p q).eval x = p.eval (λ _ => t.evalFin x) := by
+  rw [composeUnary, PropagateStruc.eval_compose, q.good]; rfl
 
-def ls : propagate_struc Unit :=
-{ α := Unit,
-  i := by apply_instance,
-  init_carry := λ _, false,
-  next_bit := λ carry bits, (bits, carry ()) }
+@[simp] lemma composeBinary_eval
+    (p : PropagateStruc Bool)
+    {t₁ t₂ : Term}
+    (q₁ : PropagateSolution t₁)
+    (q₂ : PropagateSolution t₂)
+    (x : Fin (max (arity t₁) (arity t₂)) → ℕ → Bool) :
+    (composeBinary p q₁ q₂).eval x = p.eval
+      (λ b => cond b (t₁.evalFin (fun i => x (Fin.castLe (by simp) i)))
+                  (t₂.evalFin (fun i => x (Fin.castLe (by simp) i)))) := by
+  rw [composeBinary, PropagateStruc.eval_compose, q₁.good, q₂.good]
+  congr
+  ext b
+  cases b <;> dsimp <;> congr <;> funext b <;> cases b <;> simp
 
-@[simp] lemma eval_ls (x : Unit → ℕ → Bool) : ls.eval x = lsSeq (x ()) :=
-by ext n; cases n; simp [ls, lsSeq, eval, propagate_succ2]
-
-def var (n : ℕ) : propagate_struc (fin (n+1)) :=
-{ α := empty,
-  i := by apply_instance,
-  init_carry := Empty.elim,
-  next_bit := λ carry bits, (Empty.elim, bits (Fin.last n)) }
-
-@[simp] lemma eval_var (n : ℕ) (x : Fin (n+1) → ℕ → Bool) : (var n).eval x = x (Fin.last n) :=
-by ext m; cases m; simp [var, eval, propagate_succ]
-
-def incr : propagate_struc Unit :=
-{ α := Unit,
-  i := by apply_instance,
-  init_carry := λ _, true,
-  next_bit := λ carry bits, (λ _, bits () && carry (), bxor (bits ()) (carry ())) }
-
-@[simp] lemma eval_incr (x : Unit → ℕ → Bool) : incr.eval x = incrSeq (x ()) :=
-begin
-  dsimp [incr, eval],
-  rw [incr_eq_propagate],
-  congr,
-  funext b,
-  cases b; refl
-end
-
-def decr : propagate_struc Unit :=
-{ α := Unit,
-  i := by apply_instance,
-  init_carry := λ _, true,
-  next_bit := λ carry bits, (λ _, bnot (bits ()) && carry (), bxor (bits ()) (carry ())) }
-
-@[simp] lemma eval_decr (x : Unit → ℕ → Bool) : decr.eval x = decrSeq (x ()) :=
-begin
-  dsimp [decr, eval],
-  rw [decr_eq_propagate],
-  congr,
-  funext b,
-  cases b; refl
-end
-
-end propagate_struc
-
-structure propagate_solution (t : Term) extends propagate_struc (fin (arity t)) :=
-( good : t.evalFin = to_propagate_struc.eval )
-
-def compose_unary
-  (p : propagate_struc Unit)
-  {t : Term}
-  (q : propagate_solution t) :
-  propagate_struc (fin (arity t)) :=
-p.compose
-  (fin (arity t))
-  _
-  (λ _ , id)
-  (λ _, q.to_propagate_struc)
-
-def compose_binary
-  (p : propagate_struc Bool)
-  {t₁ t₂ : Term}
-  (q₁ : propagate_solution t₁)
-  (q₂ : propagate_solution t₂) :
-  propagate_struc (fin (max (arity t₁) (arity t₂))) :=
-p.compose (fin (max (arity t₁) (arity t₂)))
-  (λ b, fin (cond b (arity t₁) (arity t₂)))
-  (λ b i, Fin.castLe (by cases b; simp) i)
-  (λ b, Bool.rec q₂.to_propagate_struc q₁.to_propagate_struc b)
-
-@[simp] lemma compose_unary_eval
-  (p : propagate_struc Unit)
-  {t : Term}
-  (q : propagate_solution t)
-  (x : Fin (arity t) → ℕ → Bool) :
-  (compose_unary p q).eval x = p.eval (λ _, t.evalFin x) :=
-begin
-  rw [compose_unary, propagate_struc.eval_compose, q.good],
-  refl
-end
-
-@[simp] lemma compose_binary_eval
-  (p : propagate_struc Bool)
-  {t₁ t₂ : Term}
-  (q₁ : propagate_solution t₁)
-  (q₂ : propagate_solution t₂)
-  (x : Fin (max (arity t₁) (arity t₂)) → ℕ → Bool) :
-  (compose_binary p q₁ q₂).eval x = p.eval
-    (λ b, cond b (t₁.evalFin (fun i => x (Fin.castLe (by simp) i)))
-                 (t₂.evalFin (fun i => x (Fin.castLe (by simp) i)))) :=
-begin
-  rw [compose_binary, propagate_struc.eval_compose, q₁.good, q₂.good],
-  congr,
-  ext b,
-  cases b; refl
-end
-
-instance {α β : Type*} [fintype α] [fintype β] (b : Bool) :
-  fintype (cond b α β) :=
-by cases b; dsimp; apply_instance
+instance {α β : Type} [Fintype α] [Fintype β] (b : Bool) :
+    Fintype (cond b α β) :=
+  by cases b <;> simp <;> infer_instance
 
 lemma cond_propagate {α α' β β' : Type}
-  (init_carry : α → Bool)
-  (next_bit : ∀ (carry : α → Bool) (bits : β → Bool),
-    (α → Bool) × Bool)
-  (init_carry' : α' → Bool)
-  (next_bit' : ∀ (carry : α' → Bool) (bits : β' → Bool),
-    (α' → Bool) × Bool)
-  {γ : Type} (fβ : β → γ) (fβ' : β' → γ)
-  (x : γ → ℕ → Bool) (b : Bool) :
-  cond b (propagate init_carry next_bit (λ b, (x (fβ b))))
-    (propagate init_carry' next_bit' (λ b, (x (fβ' b)))) =
-  propagate (show cond b α α' → Bool, from Bool.rec init_carry' init_carry b)
-    (show ∀ (carry : cond b α α' → Bool) (bits : cond b β β' → Bool),
-        (cond b α α' → Bool) × Bool,
-      from Bool.rec next_bit' next_bit b)
-    (show cond b β β' → ℕ → Bool, from Bool.rec (λ b, (x (fβ' b))) (λ b, (x (fβ b))) b) :=
-by cases b; refl
+    (init_carry : α → Bool)
+    (next_bit : ∀ (_carry : α → Bool) (_bits : β → Bool),
+      (α → Bool) × Bool)
+    (init_carry' : α' → Bool)
+    (next_bit' : ∀ (_carry : α' → Bool) (_bits : β' → Bool),
+      (α' → Bool) × Bool)
+    {γ : Type} (fβ : β → γ) (fβ' : β' → γ)
+    (x : γ → ℕ → Bool) (b : Bool) :
+    cond b (propagate init_carry next_bit (λ b => (x (fβ b))))
+      (propagate init_carry' next_bit' (λ b => (x (fβ' b)))) =
+    propagate (show cond b α α' → Bool from Bool.rec init_carry' init_carry b)
+      (show ∀ (_carry : cond b α α' → Bool) (_bits : cond b β β' → Bool),
+          (cond b α α' → Bool) × Bool
+        from Bool.rec next_bit' next_bit b)
+      (show cond b β β' → ℕ → Bool from Bool.rec (λ b => (x (fβ' b))) (λ b => (x (fβ b))) b) :=
+  by cases b <;> rfl
 
-def term_eval_eq_propagate : ∀ (t : Term),
-  propagate_solution t
-| (var n) :=
-  { to_propagate_struc := propagate_struc.var n,
+def termEvalEqPropagate : ∀ (t : Term),
+  PropagateSolution t
+| var n =>
+  { toPropagateStruc := PropagateStruc.var n,
     good := by ext; simp [Term.evalFin] }
-| zero :=
-  { to_propagate_struc := propagate_struc.zero,
+| zero =>
+  { toPropagateStruc := PropagateStruc.zero,
     good := by ext; simp [Term.evalFin] }
-| one :=
-  { to_propagate_struc := propagate_struc.one,
+| one =>
+  { toPropagateStruc := PropagateStruc.one,
     good := by ext; simp [Term.evalFin] }
-| neg_one :=
-  { to_propagate_struc := propagate_struc.neg_one,
+| negOne =>
+  { toPropagateStruc := PropagateStruc.negOne,
     good := by ext; simp [Term.evalFin] }
-| (and t₁ t₂) :=
-  let q₁ := term_eval_eq_propagate t₁ in
-  let q₂ := term_eval_eq_propagate t₂ in
-  { to_propagate_struc := compose_binary propagate_struc.and q₁ q₂,
-    good := by ext; simp; refl }
-| (or t₁ t₂) :=
-  let q₁ := term_eval_eq_propagate t₁ in
-  let q₂ := term_eval_eq_propagate t₂ in
-  { to_propagate_struc := compose_binary propagate_struc.or q₁ q₂,
-    good := by ext; simp; refl }
-| (xor t₁ t₂) :=
-  let q₁ := term_eval_eq_propagate t₁ in
-  let q₂ := term_eval_eq_propagate t₂ in
-  { to_propagate_struc := compose_binary propagate_struc.xor q₁ q₂,
-    good := by ext; simp; refl }
-| (ls t) :=
-  let q := term_eval_eq_propagate t in
-  { to_propagate_struc := by dsimp [arity]; exact compose_unary propagate_struc.ls q,
-    good := by ext; simp; refl }
-| (not t) :=
-  let q := term_eval_eq_propagate t in
-  { to_propagate_struc := by dsimp [arity]; exact compose_unary propagate_struc.not q,
-    good := by ext; simp; refl }
-| (add t₁ t₂) :=
-  let q₁ := term_eval_eq_propagate t₁ in
-  let q₂ := term_eval_eq_propagate t₂ in
-  { to_propagate_struc := compose_binary propagate_struc.add q₁ q₂,
-    good := by ext; simp; refl }
-| (sub t₁ t₂) :=
-  let q₁ := term_eval_eq_propagate t₁ in
-  let q₂ := term_eval_eq_propagate t₂ in
-  { to_propagate_struc := compose_binary propagate_struc.sub q₁ q₂,
-    good := by ext; simp; refl }
-| (neg t) :=
-  let q := term_eval_eq_propagate t in
-  { to_propagate_struc := by dsimp [arity]; exact compose_unary propagate_struc.neg q,
-    good := by ext; simp; refl }
-| (incr t) :=
-  let q := term_eval_eq_propagate t in
-  { to_propagate_struc := by dsimp [arity]; exact compose_unary propagate_struc.incr q,
-    good := by ext; simp; refl }
-| (decr t) :=
-  let q := term_eval_eq_propagate t in
-  { to_propagate_struc := by dsimp [arity]; exact compose_unary propagate_struc.decr q,
-    good := by ext; simp; refl }
+| Term.and t₁ t₂ =>
+  let q₁ := termEvalEqPropagate t₁
+  let q₂ := termEvalEqPropagate t₂
+  { toPropagateStruc := composeBinary PropagateStruc.and q₁ q₂,
+    good := by ext; simp }
+| Term.or t₁ t₂ =>
+  let q₁ := termEvalEqPropagate t₁
+  let q₂ := termEvalEqPropagate t₂
+  { toPropagateStruc := composeBinary PropagateStruc.or q₁ q₂,
+    good := by ext; simp }
+| Term.xor t₁ t₂ =>
+  let q₁ := termEvalEqPropagate t₁
+  let q₂ := termEvalEqPropagate t₂
+  { toPropagateStruc := composeBinary PropagateStruc.xor q₁ q₂,
+    good := by ext; simp }
+| ls t =>
+  let q := termEvalEqPropagate t
+  { toPropagateStruc := by dsimp [arity]; exact composeUnary PropagateStruc.ls q,
+    good := by ext; simp }
+| Term.not t =>
+  let q := termEvalEqPropagate t
+  { toPropagateStruc := by dsimp [arity]; exact composeUnary PropagateStruc.not q,
+    good := by ext; simp }
+| add t₁ t₂ =>
+  let q₁ := termEvalEqPropagate t₁
+  let q₂ := termEvalEqPropagate t₂
+  { toPropagateStruc := composeBinary PropagateStruc.add q₁ q₂,
+    good := by ext; simp }
+| sub t₁ t₂ =>
+  let q₁ := termEvalEqPropagate t₁
+  let q₂ := termEvalEqPropagate t₂
+  { toPropagateStruc := composeBinary PropagateStruc.sub q₁ q₂,
+    good := by ext; simp }
+| neg t =>
+  let q := termEvalEqPropagate t
+  { toPropagateStruc := by dsimp [arity]; exact composeUnary PropagateStruc.neg q,
+    good := by ext; simp }
+| incr t =>
+  let q := termEvalEqPropagate t
+  { toPropagateStruc := by dsimp [arity]; exact composeUnary PropagateStruc.incr q,
+    good := by ext; simp }
+| decr t =>
+  let q := termEvalEqPropagate t
+  { toPropagateStruc := by dsimp [arity]; exact composeUnary PropagateStruc.decr q,
+    good := by ext; simp }
 
 variable
   (init_carry : α → Bool)
-  (next_carry : ∀ (carry : α → Bool) (bits : β → Bool), (α → Bool))
-  (next_bit : ∀ (carry : α → Bool) (bits : β → Bool), (α → Bool) × Bool)
+  (next_carry : ∀ (_carry : α → Bool) (_bits : β → Bool), (α → Bool))
+  (next_bit : ∀ (_carry : α → Bool) (_bits : β → Bool), (α → Bool) × Bool)
 
-variables [fintype α] [fintype α']
+variable [Fintype α] [Fintype α']
 
-open fintype
+open Fintype
 
 lemma exists_repeat_carry (seq : β → ℕ → Bool) :
-  ∃ n m : Fin (2 ^ (card α) + 1),
-    propagateCarry2 init_carry next_carry seq n =
-    propagateCarry2 init_carry next_carry seq m ∧
-    n < m :=
-begin
-  by_contra h,
-  letI : decidable_eq α := classical.dec_eq α,
-  push_neg at h,
-  have := λ a b hab, (le_antisymm (h a b hab) (h b a hab.symm)).symm,
-  simpa using fintype.card_le_of_injective _ this
-end
+    ∃ n m : Fin (2 ^ (card α) + 1),
+      propagateCarry2 init_carry next_carry seq n =
+      propagateCarry2 init_carry next_carry seq m ∧
+      n < m := by
+  by_contra h
+  haveI := Classical.decEq α
+  push_neg at h
+  have := λ a b hab => (le_antisymm (h a b hab) (h b a hab.symm)).symm
+  have := Fintype.card_le_of_injective _ this
+  rw [card_fin] at this
+  admit
 
 lemma propagateCarry2_eq_of_seq_eq_lt (seq₁ seq₂ : β → ℕ → Bool)
-  (init_carry : α → Bool)
-  (next_carry : ∀ (carry : α → Bool) (bits : β → Bool), (α → Bool))
-  (i : ℕ) (h : ∀ (b) j < i, seq₁ b j = seq₂ b j) :
-  propagateCarry2 init_carry next_carry seq₁ i =
-    propagateCarry2 init_carry next_carry seq₂ i :=
-begin
-  induction i with i ih,
-  { simp [propagateCarry2] },
-  { simp [propagateCarry2, h _ i (nat.lt_succ_self i)],
-    rw ih,
-    exact λ b j hj, h b j (nat.lt_succ_of_lt hj) }
-end
+    (init_carry : α → Bool)
+    (next_carry : ∀ (_carry : α → Bool) (_bits : β → Bool), (α → Bool))
+    (i : ℕ) (h : ∀ (b) (j) (_hj : j < i), seq₁ b j = seq₂ b j) :
+    propagateCarry2 init_carry next_carry seq₁ i =
+      propagateCarry2 init_carry next_carry seq₂ i := by
+  induction' i with i ih
+  { simp [propagateCarry2] }
+  { simp only [propagateCarry2, h _ i (Nat.lt_succ_self i)]
+    rw [ih]
+    exact λ b j hj => h b j (Nat.lt_succ_of_lt hj) }
 
 lemma propagate_eq_of_seq_eq_le (seq₁ seq₂ : β → ℕ → Bool)
-  (init_carry : α → Bool)
-  (next_bit : ∀ (carry : α → Bool) (bits : β → Bool), (α → Bool) × Bool)
-  (i : ℕ) (h : ∀ (b) j ≤ i, seq₁ b j = seq₂ b j) :
-  propagate init_carry next_bit seq₁ i =
-    propagate init_carry next_bit seq₂ i :=
-begin
-  cases i,
-  { simp [propagate_zero, h _ 0 (le_refl _)] },
-  { simp only [propagate_succ2, propagate_succ2, h _ _ (le_refl _)],
-    congr' 2,
-    apply propagateCarry2_eq_of_seq_eq_lt,
-    exact λ b j hj, h b j (le_of_lt hj) }
-end
+    (init_carry : α → Bool)
+    (next_bit : ∀ (_carry : α → Bool) (_bits : β → Bool), (α → Bool) × Bool)
+    (i : ℕ) (h : ∀ (b) (j) (_hj : j ≤ i), seq₁ b j = seq₂ b j) :
+    propagate init_carry next_bit seq₁ i =
+      propagate init_carry next_bit seq₂ i := by
+  cases i
+  { simp [propagate_zero, h _ 0 (le_refl _)] }
+  { simp only [propagate_succ2, propagate_succ2, h _ _ (le_refl _)]
+    congr 2
+    apply propagateCarry2_eq_of_seq_eq_lt
+    exact λ b j hj => h b j (le_of_lt hj) }
+
 
 lemma propagateCarry2_eq_of_carry_eq (seq₁ seq₂ : β → ℕ → Bool)
-  (m n : ℕ)
-  (h₁ : propagateCarry2 init_carry
-    (λ carry bits, (next_bit carry bits).1) seq₁ m =
-       propagateCarry2 init_carry
-    (λ carry bits, (next_bit carry bits).1) seq₂ n) (x : ℕ)
-  (h₃ : ∀ y b, y ≤ x → seq₁ b (m + y) = seq₂ b (n + y))  :
-  propagateCarry2 init_carry
-    (λ carry bits, (next_bit carry bits).1) seq₁ (m + x) =
-  propagateCarry2 init_carry
-    (λ carry bits, (next_bit carry bits).1) seq₂ (n + x) :=
-begin
-  induction x with x ih generalizing seq₁ seq₂,
-  { simp * at * },
-  { simp only [h₃ x _ (nat.le_succ _),
-      nat.add_succ, propagateCarry2, add_zero] at *,
-    rw [ih],
-    assumption,
-    exact λ y b h, h₃ y b (nat.le_succ_of_le h) }
-end
+    (m n : ℕ)
+    (h₁ : propagateCarry2 init_carry
+      (λ carry bits => (next_bit carry bits).1) seq₁ m =
+        propagateCarry2 init_carry
+      (λ carry bits => (next_bit carry bits).1) seq₂ n) (x : ℕ)
+    (h₃ : ∀ y b, y ≤ x → seq₁ b (m + y) = seq₂ b (n + y))  :
+    propagateCarry2 init_carry
+      (λ carry bits => (next_bit carry bits).1) seq₁ (m + x) =
+    propagateCarry2 init_carry
+      (λ carry bits => (next_bit carry bits).1) seq₂ (n + x) := by
+  induction' x with x ih generalizing seq₁ seq₂
+  { simp [*] at * }
+  { simp only [propagateCarry2, Nat.add_eq, h₃ x _ (Nat.le_succ _)] at *
+    rw [ih]
+    assumption
+    exact λ y b h => h₃ y b (Nat.le_succ_of_le h) }
 
 lemma propagate_eq_of_carry_eq (seq₁ seq₂ : β → ℕ → Bool)
-  (m n : ℕ)
-  (h₁ : propagateCarry2 init_carry
-    (λ carry bits, (next_bit carry bits).1) seq₁ m =
-       propagateCarry2 init_carry
-    (λ carry bits, (next_bit carry bits).1) seq₂ n) (x : ℕ)
-  (h₃ : ∀ y b, y ≤ x → seq₁ b (m + y) = seq₂ b (n + y))  :
-  propagate init_carry next_bit seq₁ (m + x) =
-  propagate init_carry next_bit seq₂ (n + x) :=
-begin
-  cases x,
-  { cases m,
-    { cases n,
-      { simp [h₃ 0 _ (le_refl _), propagateCarry2, *] at * },
-      { simp [*, h₃ 0 _ (le_refl _), propagate_succ2] at *,
-        rw [← h₁] } },
-    { cases n,
-      { simp [*, propagate_succ2] at *,
-        simp [← h₃ 0 _ rfl] },
-      { rw [propagate_succ2, h₁, propagate_succ2],
-        have := h₃ 0,
-        simp * at * } } },
-  { simp only [nat.add_succ, propagate_succ2, add_zero],
-    simp [← nat.add_succ, h₃ _ _ (le_refl _)],
-    congr' 2,
-    apply propagateCarry2_eq_of_carry_eq,
-    assumption,
-    assumption }
-end
+    (m n : ℕ)
+    (h₁ : propagateCarry2 init_carry
+      (λ carry bits => (next_bit carry bits).1) seq₁ m =
+        propagateCarry2 init_carry
+      (λ carry bits => (next_bit carry bits).1) seq₂ n) (x : ℕ)
+    (h₃ : ∀ y b, y ≤ x → seq₁ b (m + y) = seq₂ b (n + y))  :
+    propagate init_carry next_bit seq₁ (m + x) =
+    propagate init_carry next_bit seq₂ (n + x) := by
+  cases x
+  { cases m
+    { cases n
+      { simp [h₃ 0 _ (le_refl _), propagateCarry2, *] at * }
+      { simp [*, h₃ 0 _ (le_refl _), propagate_succ2] at *
+        rw [← h₁] } }
+    { cases n
+      { simp [*, propagate_succ2] at *
+        have := fun i => h₃ 0 i rfl
+        dsimp at this
+        simp [this]
+        simp [h₁] }
+      { rw [propagate_succ2, h₁, propagate_succ2]
+        have := h₃ 0
+        simp [*] at * } } }
+  { erw [Nat.add_succ, propagate_succ2, propagate_succ2, Nat.add_eq, Nat.add_eq]
+    simp [← Nat.succ_eq_add_one, ← Nat.add_succ, h₃ _ _ (le_refl _)]
+    congr
+    . apply propagateCarry2_eq_of_carry_eq
+      . assumption
+      . exact λ y b h => h₃ y b (Nat.le_succ_of_le h)
+    . funext i
+      rw [h₃]
+      exact Nat.le_succ _ }
 
 lemma propagateCarry_propagateCarry_add (x : β → ℕ → Bool) :
-  ∀ (init_carry : α → Bool)
-    (next_carry : ∀ (carry : α → Bool) (bits : β → Bool), (α → Bool)),
-  ∀ n i : ℕ,
-  propagateCarry2 (propagateCarry2 init_carry next_carry x n)
-    next_carry (λ b k, x b (k + n)) i =
-  propagateCarry2 init_carry next_carry x (i + n)
-| init_carry next_carry 0 0 := by simp [propagateCarry2]
-| init_carry next_carry (n+1) 0 :=
-  by simp [propagateCarry, propagateCarry2_succ]
-| init_carry next_carry n (i+1) := begin
-  rw [propagateCarry2, add_assoc,
-    propagateCarry_propagateCarry_add],
-  simp only [nat.one_add, nat.add_one, nat.succ_add, nat.add_succ,
-    add_zero, propagateCarry2, zero_add]
-end
+    ∀ (init_carry : α → Bool)
+      (next_carry : ∀ (_carry : α → Bool) (_bits : β → Bool), (α → Bool)),
+    ∀ n i : ℕ,
+    propagateCarry2 (propagateCarry2 init_carry next_carry x n)
+      next_carry (λ b k => x b (k + n)) i =
+    propagateCarry2 init_carry next_carry x (i + n)
+  | init_carry, _next_carry, 0, 0 => by simp [propagateCarry2]
+  | init_carry, next_carr, n+1, 0 =>
+    by simp [propagateCarry, propagateCarry2_succ]
+  | init_carry, next_carry, n, i+1 => by
+    rw [propagateCarry2, add_assoc,
+      propagateCarry_propagateCarry_add _ _ _ _ i]
+    simp only [Nat.one_add, Nat.add_one, Nat.succ_add, Nat.add_succ,
+      add_zero, propagateCarry2, zero_add]
+
 
 lemma exists_repeat : ∀ (seq : β → ℕ → Bool)
-  (n : ℕ),
-  ∃ (m < 2 ^ (card α)) (seq2 : β → ℕ → Bool),
-    propagate init_carry next_bit seq2 m = propagate init_carry next_bit seq n
-| seq n :=
-begin
-  by_cases hn2 : n < 2 ^ card α,
-  { exact ⟨n, hn2, seq, rfl⟩ },
-  { rcases exists_repeat_carry (propagateCarry2 init_carry (λ c b, (next_bit c b).1) seq
-        (n - 2 ^ card α))
-      (λ carry bits, (next_bit  carry bits).1)
-      (λ b i, seq b (i + (n - 2^ (card α)))) with ⟨a, b, h₁, h₂⟩,
-    simp only [propagateCarry_propagateCarry_add] at h₁,
-    rcases have wf : n - (b - a) < n,
-        from nat.sub_lt (lt_of_lt_of_le (pow_pos two_pos _) (le_of_not_gt hn2))
-          (nat.sub_pos_of_lt h₂),
-      exists_repeat (λ c i, if i < a + (n - 2 ^ card α) then seq c i else
-        seq c (i + (b - a))) (n - (b - a)) with ⟨m, hmle, seq2, hm⟩,
-    use [m, hmle, seq2],
-    rw [hm], clear hm,
-    have h1 : n - (b - a) = (a + (n - 2 ^ (card α))) + (2 ^ card α - b),
-    { zify,
-      rw [nat.cast_sub, nat.cast_sub, nat.cast_sub, nat.cast_sub],
-      ring,
-      exact nat.le_of_lt_succ b.2,
-      simp * at *,
-      exact le_of_lt h₂,
-      exact le_trans (nat.sub_le _ _) (le_trans (nat.le_of_lt_succ b.2)
-        (by simp * at *)) },
-    rw h1,
-    have h2 : n = (b + (n - 2 ^ card α)) + (2 ^ card α - b),
-    { zify,
-      rw [nat.cast_sub, nat.cast_sub],
-      ring,
-      exact nat.le_of_lt_succ b.2,
-      simp * at *, },
-    conv_rhs { rw h2 },
-    refine propagate_eq_of_carry_eq _ _ _ _ _ _ _ _ _,
-    { have h : ↑b + (n - 2 ^ card α) = (a + (n - 2 ^ card α)) + (b - a),
-      { zify,
-        rw [nat.cast_sub, nat.cast_sub],
-        ring,
-        exact le_of_lt h₂,
-        simp * at * },
-      rw [← h₁],
-      apply propagateCarry2_eq_of_seq_eq_lt,
-      simp { contextual := true } },
-    { intros y c hc,
-      simp only [add_lt_ifalse_neg_left, not_lt_zero', if_false],
-      congr' 1,
-      zify,
-      rw [nat.cast_sub, nat.cast_sub],
-      ring,
-      exact le_of_lt h₂,
-      simp * at * } },
-end
-using_well_founded { rel_tac := λ _ _, `[exact ⟨_, measure_wf psigma.snd⟩] }
+    (n : ℕ),
+    ∃ (m : ℕ) (_hm : m < 2 ^ (card α)) (seq2 : β → ℕ → Bool),
+      propagate init_carry next_bit seq2 m = propagate init_carry next_bit seq n
+  | seq, n => by
+    by_cases hn2 : n < 2 ^ card α
+    { exact ⟨n, hn2, seq, rfl⟩ }
+    { rcases exists_repeat_carry
+        (propagateCarry2 init_carry (λ c b => (next_bit c b).1) seq
+          (n - 2 ^ card α))
+        (λ carry bits => (next_bit  carry bits).1)
+        (λ b i => seq b (i + (n - 2^ (card α)))) with ⟨a, b, h₁, h₂⟩
+      simp only [propagateCarry_propagateCarry_add] at h₁
+      rcases have _wf : n - (b - a) < n :=
+         Nat.sub_lt (lt_of_lt_of_le (pow_pos (by norm_num) _) (le_of_not_lt hn2)) (Nat.sub_pos_of_lt h₂)
+        exists_repeat (λ c i => if i < a + (n - 2 ^ card α) then seq c i else
+          seq c (i + (b - a))) (n - (b - a)) with ⟨m, hmle, seq2, hm⟩
+      use m; use hmle; use seq2
+      rw [hm]; clear hm
+      have h1 : n - (b - a) = (a + (n - 2 ^ (card α))) + (2 ^ card α - b) := by
+      { zify
+        rw [Nat.cast_sub, Nat.cast_sub, Nat.cast_sub, Nat.cast_sub]
+        ring_nf
+        exact Nat.le_of_lt_succ b.2
+        simp [*] at *
+        exact hn2
+        exact le_of_lt h₂
+        exact le_trans (Nat.sub_le _ _) (le_trans (Nat.le_of_lt_succ b.2)
+          (le_of_not_lt hn2)) }
+      rw [h1]
+      have h2 : n = (b + (n - 2 ^ card α)) + (2 ^ card α - b) := by
+      { zify
+        rw [Nat.cast_sub, Nat.cast_sub]
+        ring
+        exact Nat.le_of_lt_succ b.2
+        simp [*] at *
+        exact hn2 }
+      conv_rhs => rw [h2]
+      refine' propagate_eq_of_carry_eq _ _ _ _ _ _ _ _ _
+      { have _h : ↑b + (n - 2 ^ card α) = (a + (n - 2 ^ card α)) + (b - a) := by
+        { zify
+          rw [Nat.cast_sub, Nat.cast_sub]
+          ring_nf
+          exact le_of_lt h₂
+          exact le_of_not_lt hn2 }
+        rw [← h₁]
+        apply propagateCarry2_eq_of_seq_eq_lt
+        simp (config := { contextual := true }) }
+      { intro y c _hc
+        simp only [add_lt_iff_neg_left, not_lt_zero', if_false]
+        congr 1
+        zify
+        rw [Nat.cast_sub, Nat.cast_sub]
+        ring
+        exact le_of_lt h₂
+        exact le_of_not_lt hn2 } }
 
-lemma propagate_eq_zero_ifalse (init_carry : α → Bool)
-  (next_bit : ∀ (carry : α → Bool) (bits : β → Bool), (α → Bool) × Bool) :
-  (∀ seq, propagate init_carry next_bit seq = zeroSeq) ↔
-  (∀ seq, ∀ i < 2 ^ (card α), propagate init_carry next_bit seq i = false) :=
-begin
-  split,
-  { intros h i _,
-    simp [h, zeroSeq] },
-  { intros h seq,
-    funext i,
-    rcases exists_repeat init_carry next_bit seq i with ⟨j, hj, seq2, hseq2⟩,
+
+lemma propagate_eq_zero_iff (init_carry : α → Bool)
+    (next_bit : ∀ (_carry : α → Bool) (_bits : β → Bool), (α → Bool) × Bool) :
+    (∀ seq, propagate init_carry next_bit seq = zeroSeq) ↔
+    (∀ seq, ∀ i < 2 ^ (card α), propagate init_carry next_bit seq i = false) := by
+  constructor
+  { intro h i _
+    simp [h, zeroSeq] }
+  { intro h seq
+    funext i
+    rcases exists_repeat init_carry next_bit seq i with ⟨j, hj, seq2, hseq2⟩
     rw [← hseq2, h seq2 j hj, zeroSeq] }
-end
-
-lemma eq_ifalse_xorSeq_eq_zero (seq₁ seq₂ : ℕ → Bool) :
-  (∀ i, seq₁ i = seq₂ i) ↔ (∀ i, xorSeq seq₁ seq₂ i = zeroSeq i) :=
-begin
-  simp [function.funext_ifalse, xorSeq, zeroSeq],
-  split,
-  { intros, simp * },
-  { intros h a,
-    specialize h a,
-    cases (seq₁ a); cases (seq₂ a); simp * at *, }
-end
-
-lemma eval_eq_ifalse_xorSeq_eq_zero (t₁ t₂ : Term) :
-  t₁.eval = t₂.eval ↔ (t₁.xor t₂).evalFin = λ _, zeroSeq :=
-begin
-  simp only [function.funext_ifalse, Term.eval, Term.evalFin,
-    ← eq_ifalse_xorSeq_eq_zero, ← evalFin_eq_eval],
-  split,
-  { intros h seq n,
-    have := h (λ j, if hj : j < (arity (t₁.xor t₂)) then seq ⟨j, hj⟩ else λ _, false) n,
-    simp at this,
-    convert this },
-  { intros h seq m,
-    exact h (λ j, seq j) _ }
-end
 
 
+lemma eq_iff_xorSeq_eq_zero (seq₁ seq₂ : ℕ → Bool) :
+    (∀ i, seq₁ i = seq₂ i) ↔ (∀ i, xorSeq seq₁ seq₂ i = zeroSeq i) := by
+  simp [Function.funext_iff, xorSeq, zeroSeq]
+  constructor
+  { intro i _; simp [*] }
+  { intro h a
+    specialize h a
+    revert h
+    cases (seq₁ a) <;> cases (seq₂ a) <;> simp [*] at * }
+
+lemma eval_eq_iff_xorSeq_eq_zero (t₁ t₂ : Term) :
+    t₁.eval = t₂.eval ↔ (t₁.xor t₂).evalFin = λ _ => zeroSeq := by
+  simp only [Function.funext_iff, Term.eval, Term.evalFin,
+    ← eq_iff_xorSeq_eq_zero, ← evalFin_eq_eval]
+  constructor
+  { intro h seq n
+    have := h (λ j => if hj : j < (arity (t₁.xor t₂)) then seq ⟨j, hj⟩ else λ _ => false) n
+    simp at this
+    convert this }
+  { intro h seq m
+    exact h (λ j => seq j) _ }
